Update till exh_to_patProof
For #244 and #245. Also attempt to improve do_app-related theorems.

compiler/backend/semantics/patSemScript.sml
@@ -111,6 +111,25 @@ val _ = Define `
   ∧
   (v_to_char_list _ = NONE)`;
 
+val vs_to_w8s_def = Define`
+  (vs_to_w8s s [] = SOME []) ∧
+  (vs_to_w8s s (Loc l::vs) =
+   case store_lookup l s of
+   | SOME (W8array ws1) =>
+     (case vs_to_w8s s vs of
+      | SOME ws2 => SOME (ws1++ws2)
+      | _ => NONE)
+   | _ => NONE) ∧
+  (vs_to_w8s _ _ = NONE)`;
+
+val vs_to_string_def = Define`
+  (vs_to_string [] = SOME "") ∧
+  (vs_to_string (Litv(StrLit s1)::vs) =
+   case vs_to_string vs of
+   | SOME s2 => SOME (s1++s2)
+   | _ => NONE) ∧
+  (vs_to_string _ = NONE)`;
+
 val _ = Define `
   Boolv b = Conv (if b then true_tag else false_tag) []`;
 
@@ -209,12 +228,31 @@ val do_app_def = Define `
                   )
         | _ => NONE
         )
+    | (Op (Op Aw8concat), [v]) =>
+      (case v_to_list v of
+        SOME vs =>
+          (case vs_to_w8s s.refs vs of
+            SOME ws =>
+              let (s',lnum) = (store_alloc (W8array ws) s.refs)
+              in SOME (s with refs := s', Rval (Loc lnum))
+            | _ => NONE)
+        | _ => NONE)
     | (Op (Op (WordFromInt wz)), [Litv (IntLit i)]) =>
       SOME (s, Rval (Litv (do_word_from_int wz i)))
     | (Op (Op (WordToInt wz)), [Litv w]) =>
       (case do_word_to_int wz w of
         | NONE => NONE
         | SOME i => SOME (s, Rval (Litv (IntLit i))))
+    | (Op (Op StrFromW8Array), [Loc lnum]) =>
+        (case store_lookup lnum s.refs of
+          SOME (W8array ws) =>
+            SOME (s, Rval (Litv(StrLit(MAP (CHR o w2n) ws))))
+        | _ => NONE)
+    | (Op (Op StrToW8Array), [Litv(StrLit str)]) =>
+        let (s',lnum) =
+          (store_alloc (W8array (MAP (n2w o ORD) str)) s.refs)
+        in
+          SOME (s with refs := s', Rval (Loc lnum))
     | (Op (Op Ord), [Litv (Char c)]) =>
           SOME (s, Rval (Litv(IntLit(int_of_num(ORD c)))))
     | (Op (Op Chr), [Litv (IntLit i)]) =>
@@ -242,6 +280,14 @@ val do_app_def = Define `
               SOME (s, Rval (Litv (Char (EL n str))))
     | (Op (Op Strlen), [Litv (StrLit str)]) =>
         SOME (s, Rval (Litv(IntLit(int_of_num(STRLEN str)))))
+    | (Op (Op Strcat), [v]) =>
+        (case v_to_list v of
+          SOME vs =>
+            (case vs_to_string vs of
+              SOME str =>
+                SOME (s, Rval (Litv(StrLit str)))
+            | _ => NONE)
+        | _ => NONE)
     | (Op (Op VfromList), [v]) =>
           (case v_to_list v of
               SOME vs =>
@@ -321,46 +367,24 @@ val do_app_def = Define `
     | _ => NONE
   )))`;
 
-val do_app_cases = Q.store_thm("do_app_cases",
-  `patSem$do_app s op vs = SOME x ⇒
-    (∃z n1 n2. op = (Op (Op (Opn z))) ∧ vs = [Litv (IntLit n1); Litv (IntLit n2)]) ∨
-    (∃z n1 n2. op = (Op (Op (Opb z))) ∧ vs = [Litv (IntLit n1); Litv (IntLit n2)]) ∨
-    (∃z wz w1 w2. op = (Op (Op (Opw wz z))) ∧ vs = [Litv w1; Litv w2]) ∨
-    (∃sh z wz w. op = (Op (Op (Shift wz sh z))) ∧ vs = [Litv w]) ∨
-    (∃v1 v2. op = (Op (Op Equality)) ∧ vs = [v1; v2]) ∨
-    (∃lnum v. op = (Op (Op Opassign)) ∧ vs = [Loc lnum; v]) ∨
-    (∃n. op = (Op (Op Opderef)) ∧ vs = [Loc n]) ∨
-    (∃v. op = (Op (Op Opref)) ∧ vs = [v]) ∨
-    (∃idx v. op = (Op (Init_global_var idx)) ∧ vs = [v]) ∨
-    (∃n l tag v. op = Tag_eq n l ∧ vs = [Conv tag v]) ∨
-    (∃n tag v. op = El n ∧ vs = [Conv tag v]) ∨
-    (∃n w. op = (Op (Op Aw8alloc)) ∧ vs = [Litv (IntLit n); Litv (Word8 w)]) ∨
-    (∃lnum i. op = (Op (Op Aw8sub)) ∧ vs = [Loc lnum; Litv (IntLit i)]) ∨
-    (∃n. op = (Op (Op Aw8length)) ∧ vs = [Loc n]) ∨
-    (∃lnum i w. op = (Op (Op Aw8update)) ∧ vs = [Loc lnum; Litv (IntLit i); Litv (Word8 w)]) ∨
-    (∃wz w. op = (Op (Op (WordToInt wz))) ∧ vs = [Litv w]) ∨
-    (∃wz n. op = (Op (Op (WordFromInt wz))) ∧ vs = [Litv (IntLit n)]) ∨
-    (∃c. op = (Op (Op Ord)) ∧ vs = [Litv (Char c)]) ∨
-    (∃n. op = (Op (Op Chr)) ∧ vs = [Litv (IntLit n)]) ∨
-    (∃z c1 c2. op = (Op (Op (Chopb z))) ∧ vs = [Litv (Char c1); Litv (Char c2)]) ∨
-    (∃s i. op = (Op (Op Strsub)) ∧ vs = [Litv (StrLit s); Litv (IntLit i)]) ∨
-    (∃v ls. op = (Op (Op Implode)) ∧ vs = [v] ∧ (v_to_char_list v = SOME ls)) ∨
-    (∃s. op = (Op (Op Strlen)) ∧ vs = [Litv (StrLit s)]) ∨
-    (∃v vs'. op = (Op (Op VfromList)) ∧ vs = [v] ∧ (v_to_list v = SOME vs')) ∨
-    (∃vs' i. op = (Op (Op Vsub)) ∧ vs = [Vectorv vs'; Litv (IntLit i)]) ∨
-    (∃vs'. op = (Op (Op Vlength)) ∧ vs = [Vectorv vs']) ∨
-    (∃v n. op = (Op (Op Aalloc)) ∧ vs = [Litv (IntLit n); v]) ∨
-    (∃lnum i. op = (Op (Op Asub)) ∧ vs = [Loc lnum; Litv (IntLit i)]) ∨
-    (∃n. op = (Op (Op Alength)) ∧ vs = [Loc n]) ∨
-    (∃lnum i v. op = (Op (Op Aupdate)) ∧ vs = [Loc lnum; Litv (IntLit i); v]) ∨
-    (∃lnum n. op = (Op (Op (FFI n))) ∧ vs = [Loc lnum])`,
-  rw[do_app_def] >>
-  pop_assum mp_tac >>
-  Cases_on`op` >- (
-    simp[] >>
-    every_case_tac >> fs[] ) >>
-  BasicProvers.CASE_TAC >>
-  every_case_tac);
+val op_thms = { nchotomy = patLangTheory.op_nchotomy, case_def = patLangTheory.op_case_def}
+val conop_thms = { nchotomy = conLangTheory.op_nchotomy, case_def = conLangTheory.op_case_def}
+val astop_thms = {nchotomy = astTheory.op_nchotomy, case_def = astTheory.op_case_def}
+val list_thms = { nchotomy = list_nchotomy, case_def = list_case_def}
+val option_thms = { nchotomy = option_nchotomy, case_def = option_case_def}
+val v_thms = { nchotomy = theorem"v_nchotomy", case_def = definition"v_case_def"}
+val sv_thms = { nchotomy = semanticPrimitivesTheory.store_v_nchotomy, case_def = semanticPrimitivesTheory.store_v_case_def }
+val lit_thms = { nchotomy = astTheory.lit_nchotomy, case_def = astTheory.lit_case_def}
+val eqs = LIST_CONJ (map prove_case_eq_thm
+  [op_thms, conop_thms, astop_thms, list_thms, option_thms, v_thms, sv_thms, lit_thms])
+
+val do_app_cases = save_thm("do_app_cases",
+  ``patSem$do_app s op vs = SOME x`` |>
+  SIMP_CONV(srw_ss()++COND_elim_ss++LET_ss)[PULL_EXISTS, do_app_def, eqs, pair_case_eq]);
+
+val do_app_cases_none = save_thm("do_app_cases_none",
+  ``patSem$do_app s op vs = NONE`` |>
+  SIMP_CONV(srw_ss()++COND_elim_ss++LET_ss)[PULL_EXISTS, do_app_def, eqs, pair_case_eq]);
 
 val do_if_def = Define `
   do_if v e1 e2 =
@@ -461,9 +485,8 @@ val evaluate_ind = theorem"evaluate_ind"
 
 val do_app_clock = Q.store_thm("do_app_clock",
   `patSem$do_app s op vs = SOME(s',r) ==> s.clock = s'.clock`,
-  rpt strip_tac
-  THEN imp_res_tac do_app_cases
-  THEN (fs [do_app_def] >> every_case_tac >> fs[LET_THM,semanticPrimitivesTheory.store_alloc_def,semanticPrimitivesTheory.store_assign_def] >> rw[]))
+  rpt strip_tac THEN fs[do_app_cases] >> every_case_tac >>
+  fs[LET_THM,semanticPrimitivesTheory.store_alloc_def,semanticPrimitivesTheory.store_assign_def] >> rw[])
 
 val evaluate_clock = Q.store_thm("evaluate_clock",
   `(∀env s1 e r s2. evaluate env s1 e = (s2,r) ⇒ s2.clock ≤ s1.clock)`,
